finished writing the Fixed Payout contract (pre-elaborated)

FixedPayout/FixedPayout.fst
@@ -14,8 +14,62 @@ module CR    = Zen.ContractResult
 module Asset = Zen.Asset
 module Opt   = Zen.Option
 
-let _cwt = ""
-let _defaultHash = Zen.Hash.Sha3.empty |> Zen.Hash.Sha3.finalize
+type ticker = s:string {FStar.String.length s <= 4}
+
+// compressed public key
+type cpk = byte ** hash
+
+type preAuditPath = p: list data{length p == 256}
+
+type auditPath = p: list hash{length p == 256}
+
+type attestation = {
+    timestamp  : timestamp;
+    commit     : hash;
+    pubKey     : publicKey;
+}
+
+type position =
+    | Bull
+    | Bear
+
+type event = {
+    oraclePubKey     : publicKey;
+    oracleContractId : contractId;
+    ticker           : ticker;
+    priceLow         : U64.t;
+    priceHigh        : option U64.t;
+    timeLow          : U64.t;
+    timeHigh         : option U64.t;
+}
+
+type bet = {
+    event    : event;
+    position : position;
+}
+
+type proof = {
+    key         : ticker;
+    value       : U64.t;
+    root        : hash;
+    auditPath   : auditPath;
+    cwt         : string;
+    defaultHash : hash;
+}
+
+type redemption = {
+    bet         : bet;
+    attestation : attestation;
+    proof       : proof;
+}
+
+
+
+(*
+-------------------------------------------------------------------------------
+========== UTILITY FUNCTIONS ==================================================
+-------------------------------------------------------------------------------
+*)
 
 // tries to map a function over a list.
 // if all of the mappings return Some, then returns Some list.
@@ -35,60 +89,6 @@ let rec tryMap #a #b #n f ls = //20
             Zen.OptionT.some result
         | _ -> Zen.OptionT.none end
     | [] -> [] |> Zen.OptionT.incSome (length ls * n)
-
-type ticker = s:string {FStar.String.length s <= 4}
-
-// compressed public key
-type cpk = byte ** hash
-
-type preAuditPath = p: list data{length p == 256}
-
-type auditPath = p: list hash{length p == 256}
-
-type attestation = {
-    timestamp : timestamp;
-    commit    : hash;
-    pubKey    : publicKey;
-}
-
-type position =
-    | Bull
-    | Bear
-
-type event = {
-    oraclePubKey : publicKey;
-    ticker       : ticker;
-    priceLow     : U64.t;
-    priceHigh    : option U64.t;
-    timeLow      : U64.t;
-    timeHigh     : option U64.t;
-}
-
-type bet = {
-    event    : event;
-    position : position;
-}
-
-type proof = {
-    key       : ticker;
-    value     : U64.t;
-    root      : hash;
-    auditPath : auditPath;
-}
-
-type redemption = {
-    bet         : bet;
-    attestation : attestation;
-    proof       : proof;
-}
-
-
-
-(*
--------------------------------------------------------------------------------
-========== UTILITY FUNCTIONS ==================================================
--------------------------------------------------------------------------------
-*)
 
 let runOpt (#a #s:Type) (#m:nat) (update:a -> s -> s `cost` m) (x:option a) (st:s): s `cost` m =
     Opt.maybe (incRet m) update x st
@@ -145,8 +145,8 @@ let parseDict data =
         |> RT.ofOptionT "Data parsing failed - the message body isn't a dictionary"
         |> RT.map Some
     | None ->
-        RT.failw "Data parsing failed - the message body is empty"
-        |> inc 4
+        "Data parsing failed - the message body is empty"
+        |> RT.incFailw 4
 
 val parseField (#a:Type) (#m:nat)
     : (data -> option a `cost` m)
@@ -158,9 +158,11 @@ let parseField #_ #_ parser fieldName errMsg dict =
     let! value = dict >!= Dict.tryFind fieldName >?= parser in
     match value with
     | Some value ->
-        RT.ok value
+        value
+        |> RT.ok
     | None ->
-        RT.autoFailw errMsg
+        errMsg
+        |> RT.failw
 
 val parseOptField (#a:Type) (#m:nat)
     : (data -> option a `cost` m)
@@ -178,7 +180,7 @@ let parseTicker fieldName errMsg dict =
     >>= (fun s ->
         if FStar.String.length s <= 4
             then let s : ticker = s in RT.ok s
-            else RT.autoFailw "Ticker size can't be bigger than 4")
+            else RT.failw "Ticker size can't be bigger than 4")
 
 val extractHashes: string -> ls:list data -> result (ls':list hash {length ls' == length ls}) `cost` (length ls * 2)
 let extractHashes errMsg ls =
@@ -198,7 +200,7 @@ let parsePreAuditPath fieldName errMsg dict =
     >>= (fun ls ->
         if length ls = 256
             then let ls : preAuditPath = ls in RT.ok ls
-            else RT.autoFailw "AuditPath length must be 256")
+            else RT.failw "AuditPath length must be 256")
 
 val parseAuditPath: string -> string -> option (Dict.t data) -> result auditPath `cost` 580
 let parseAuditPath fieldName errMsg dict =
@@ -206,14 +208,64 @@ let parseAuditPath fieldName errMsg dict =
     parsePreAuditPath fieldName errMsg dict
     >>= extractAuditPath
 
-let getTimestamp    = parseField    tryU64       "Timestamp"    "Could not parse Timestamp"
-let getCommit       = parseField    tryHash      "Commit"       "Could not parse Commit"
-let getOraclePubKey = parseField    tryPublicKey "OraclePubKey" "Could not parse OraclePubKey"
-let getTicker       = parseTicker                "Ticker"       "Could not parse Ticker"
-let getPriceLow     = parseField    tryU64       "PriceLow"     "Could not parse PriceLow"
-let getPriceHigh    = parseOptField tryU64       "PriceHigh"
-let getTimeLow      = parseField    tryU64       "TimeLow"      "Could not parse TimeLow"
-let getTimeHigh     = parseOptField tryU64       "TimeHigh"
+val parsePosition: string -> string -> option (Dict.t data) -> result position `cost` 66
+let parsePosition fieldName errMsg dict =
+    let open Zen.ResultT in
+    parseField tryString fieldName errMsg dict >>=
+    (function
+    | "Bull" -> ret Bull
+    | "Bear" -> ret Bear
+    | _      -> RT.failw "Position must be either Bull or Bear")
+
+val parseContractId: string -> string -> option (Dict.t data) -> result contractId `cost` 130
+let parseContractId fieldName errMsg dict =
+    let open Zen.ResultT in
+    parseField tryString fieldName errMsg dict >>=
+    (fun s ->
+        begin
+        if FStar.String.length s = 72
+            then
+                begin
+                let (s:string { FStar.String.length s = 72 }) = s in
+                s
+                |> Zen.ContractId.parse
+                |> Zen.ResultT.ofOptionT "OracleContractId is not a valid contractId" // 64
+                end
+            else "OracleContractId must be 72 characters long" |> RT.incFailw 64
+        end)
+
+let getTimestamp        = parseField      tryU64       "Timestamp"        "Could not parse Timestamp"
+let getCommit           = parseField      tryHash      "Commit"           "Could not parse Commit"
+let getOraclePubKey     = parseField      tryPublicKey "OraclePubKey"     "Could not parse OraclePubKey"
+let getTicker           = parseTicker                  "Ticker"           "Could not parse Ticker"
+let getPriceLow         = parseField      tryU64       "PriceLow"         "Could not parse PriceLow"
+let getPriceHigh        = parseOptField   tryU64       "PriceHigh"
+let getTimeLow          = parseField      tryU64       "TimeLow"          "Could not parse TimeLow"
+let getTimeHigh         = parseOptField   tryU64       "TimeHigh"
+let getAuditPath        = parseAuditPath               "AuditPath"        "Could not parse AuditPath"
+let getValue            = parseField      tryU64       "Value"            "Could not parse Value"
+let getCWT              = parseField      tryString    "CWT"              "Could not parse CWT"
+let getDefaultHash      = parseField      tryHash      "DefaultHash"      "Could not parse DefaultHash"
+let getPosition         = parsePosition                "Position"         "Could not parse Position"
+let getOracleContractId = parseContractId              "OracleContractId" "Could not parse OracleContractId"
+
+val parseProof: option (Dict.t data) -> result proof `cost` 910
+let parseProof dict =
+    let open Zen.ResultT in
+    dict |> getTicker      >>= (fun key         ->
+    dict |> getValue       >>= (fun value       ->
+    dict |> getCommit      >>= (fun root        ->
+    dict |> getAuditPath   >>= (fun auditPath   ->
+    dict |> getCWT         >>= (fun cwt         ->
+    dict |> getDefaultHash >>= (fun defaultHash ->
+        RT.ok ({
+            key         = key;
+            value       = value;
+            root        = root;
+            auditPath   = auditPath;
+            cwt         = cwt;
+            defaultHash = defaultHash;
+        })))))))
 
 val parseAttestation: option (Dict.t data) -> result attestation `cost` 198
 let parseAttestation dict =
@@ -227,23 +279,41 @@ let parseAttestation dict =
             pubKey    = pubKey;
         }))))
 
-val parseEvent: option (Dict.t data) -> result event `cost` 396
+val parseEvent: option (Dict.t data) -> result event `cost` 526
 let parseEvent dict =
     let open Zen.ResultT in
-    dict |> getOraclePubKey >>= (fun oraclePubKey ->
-    dict |> getTicker       >>= (fun ticker       ->
-    dict |> getPriceLow     >>= (fun priceLow     ->
-    dict |> getPriceHigh    >>= (fun priceHigh    ->
-    dict |> getTimeLow      >>= (fun timeLow      ->
-    dict |> getTimeHigh     >>= (fun timeHigh     ->
+    dict |> getOraclePubKey     >>= (fun oraclePubKey     ->
+    dict |> getOracleContractId >>= (fun oracleContractId ->
+    dict |> getTicker           >>= (fun ticker           ->
+    dict |> getPriceLow         >>= (fun priceLow         ->
+    dict |> getPriceHigh        >>= (fun priceHigh        ->
+    dict |> getTimeLow          >>= (fun timeLow          ->
+    dict |> getTimeHigh         >>= (fun timeHigh         ->
         RT.ok ({
-            oraclePubKey = oraclePubKey;
-            ticker       = ticker;
-            priceLow     = priceLow;
-            priceHigh    = priceHigh;
-            timeLow      = timeLow;
-            timeHigh     = timeHigh;
-        })))))))
+            oraclePubKey     = oraclePubKey;
+            oracleContractId = oracleContractId;
+            ticker           = ticker;
+            priceLow         = priceLow;
+            priceHigh        = priceHigh;
+            timeLow          = timeLow;
+            timeHigh         = timeHigh;
+        }))))))))
+
+val parseRedemption: option (Dict.t data) -> result redemption `cost` 1700
+let parseRedemption dict =
+    let open Zen.ResultT in
+    dict |> parseEvent       >>= (fun event       ->
+    dict |> getPosition      >>= (fun position    ->
+    dict |> parseAttestation >>= (fun attestation ->
+    dict |> parseProof       >>= (fun proof       ->
+        RT.ok ({
+            bet         = {
+                event    = event;
+                position = position;
+            };
+            attestation = attestation;
+            proof       = proof;
+        })))))
 
 
 
@@ -264,9 +334,15 @@ let updateTicker (tick:ticker) (s:Sha3.t): Sha3.t `cost` 24 =
     >>= Sha3.updateString tick
     >>= incRet (6 * (4 - FStar.String.length tick))
 
-let updateEvent (event:event) (s:Sha3.t): Sha3.t `cost` 546 =
+let updateContractId ((v,h):contractId) (s:Sha3.t): Sha3.t `cost` 216 =
+    ret s
+    >>= Sha3.updateU32 v  // 24
+    >>= Sha3.updateHash h // 192
+
+let updateEvent (event:event) (s:Sha3.t): Sha3.t `cost` 762 =
     ret s
     >>= updatePublicKey         event.oraclePubKey
+    >>= updateContractId        event.oracleContractId
     >>= updateTicker            event.ticker
     >>= Sha3.updateU64          event.priceLow
     >>= Sha3.updateU64 `runOpt` event.priceHigh
@@ -295,17 +371,17 @@ let hashAttestation (attestation:attestation): hash `cost` 802 =
     >>= Sha3.updateHash commit // 192
     >>= Sha3.finalize // 20
 
-let hashBet (bet:bet): hash `cost` 590 =
+let hashBet (bet:bet): hash `cost` 806 =
     ret Sha3.empty
     >>= updateEvent    bet.event
     >>= updatePosition bet.position
     >>= Sha3.finalize
 
-let betToken ((v, h):contractId) (bet:bet): asset `cost` 590 =
+let mkBetToken ((v, h):contractId) (bet:bet): asset `cost` 806 =
     let! betHash = hashBet bet in
     ret (v, h, betHash)
 
-let attestToken ((v,h):contractId) (attestation:attestation): asset `cost` 802 =
+let mkAttestToken ((v,h):contractId) (attestation:attestation): asset `cost` 802 =
     let! attestHash = hashAttestation attestation in
     ret (v, h, attestHash)
 
@@ -313,58 +389,77 @@ let attestToken ((v,h):contractId) (attestation:attestation): asset `cost` 802 =
 
 (*
 -------------------------------------------------------------------------------
-========== AUDIT PATH VALIDATION ==============================================
+========== VALIDATION =========================================================
 -------------------------------------------------------------------------------
 *)
 
+val inBounds : U64.t -> option U64.t -> U64.t -> bool `cost` 0
+let inBounds low high value =
+    (low `U64.lte` value && Opt.maybe true (U64.lte value) high)
+    |> ret
+
+val validateTime: redemption -> result redemption `cost` 0
+let validateTime redemption =
+    let  event = redemption.bet.event             in
+    let  low   = event.timeLow                    in
+    let  high  = event.timeHigh                   in
+    let  value = redemption.attestation.timestamp in
+    let! inb   = inBounds low high value          in
+    if inb
+        then RT.ok redemption
+        else RT.failw "Attestation time is not within the given time bounds"
+
+val validatePrice: redemption -> result redemption `cost` 0
+let validatePrice redemption =
+    let  event = redemption.bet.event    in
+    let  low   = event.priceLow          in
+    let  high  = event.priceHigh         in
+    let  value = redemption.proof.value  in
+    let! inb   = inBounds low high value in
+    let  pos   = redemption.bet.position in
+    match inb, pos with
+    | true, Bull
+    | false, Bear ->
+        RT.ok redemption
+    | _ ->
+        RT.failw "Position doesn't match the event"
 
 val hashKey : ticker -> hash `cost` 44
 let hashKey s =
     Sha3.ofString s
     |> inc (24 - (6 * FStar.String.length s))
 
-val verifyAuditPath : proof -> bool `cost` 107588
+val verifyAuditPath : proof -> bool `cost` 107568
 let verifyAuditPath proof =
-    let! defaultHash = _defaultHash in
     let! key = hashKey proof.key in
     let value = Zen.SparseMerkleTree.serializeU64 proof.value in
-    Zen.SparseMerkleTree.verify _cwt defaultHash proof.root proof.auditPath key (Some value)
+    Zen.SparseMerkleTree.verify proof.cwt proof.defaultHash proof.root proof.auditPath key (Some value)
 
+val validateAuditPath: redemption -> result redemption `cost` 107568
+let validateAuditPath redemption =
+    let! b = verifyAuditPath redemption.proof in
+    if b
+        then RT.ok redemption
+        else RT.failw "Invalid audit path"
 
-(*)
-type proof = {
-    key       : ticker;
-    value     : U64.t;
-    root      : hash;
-    auditPath : auditPath;
-}
+val validateRedemption: redemption -> result redemption `cost` 107568
+let validateRedemption =
+    let open RT in
+    ret
+    >=> validateTime
+    >=> validatePrice
+    >=> validateAuditPath
 
-val serializeU64:
-    value: FStar.UInt64.t
-    -> hash
-
--val verify:
-    cwt: string
-    -> defaultHash: hash
-    -> root: hash
-    -> auditPath: list hash
-    -> key: hash
-    -> value: option hash
-    -> bool `cost` (length auditPath * 420 + 4)
-
-
-
-(*)
 (*
 -------------------------------------------------------------------------------
 ========== COMMAND: Buy  ======================================================
 -------------------------------------------------------------------------------
 *)
 
-val buyEvent: txSkeleton -> contractId -> sender -> event -> CR.t `cost` 2203 //(590 + 590 + 64 + 64 + 64 + 414 + 414 + 3)
+val buyEvent: txSkeleton -> contractId -> sender -> event -> CR.t `cost` 2635 //(806 + 806 + 64 + 64 + 64 + 414 + 414 + 3)
 let buyEvent txSkel contractId sender event =
-    let! bullToken = betToken contractId ({event=event; position=Bull}) in // 590
-    let! bearToken = betToken contractId ({event=event; position=Bear}) in // 590
+    let! bullToken = mkBetToken contractId ({event=event; position=Bull}) in // 806
+    let! bearToken = mkBetToken contractId ({event=event; position=Bear}) in // 806
     let! m = TX.getAvailableTokens Asset.zenAsset txSkel in // 64
     ret txSkel
     >>= TX.mint m bullToken // 64
@@ -373,12 +468,12 @@ let buyEvent txSkel contractId sender event =
     >>= lockToSender bearToken m sender // 414
     >>= CR.ofTxSkel //3
 
-val buy: txSkeleton -> contractId -> sender -> option data -> CR.t `cost` 2603 //(4 + 396 + 2203)
+val buy: txSkeleton -> contractId -> sender -> option data -> CR.t `cost` 3165 //(4 + 526 + 2635)
 let buy txSkel contractId sender messageBody =
     let open RT in
     parseDict messageBody  // 4
-    >>= parseEvent // 396
-    >>= buyEvent txSkel contractId sender // 2203
+    >>= parseEvent // 526
+    >>= buyEvent txSkel contractId sender // 2635
 
 
 
@@ -388,13 +483,24 @@ let buy txSkel contractId sender messageBody =
 -------------------------------------------------------------------------------
 *)
 
-val inBounds : U64.t -> option U64.t -> U64.t -> bool `cost` 0
-let inBounds low high value =
-    (low `U64.lte` value && Opt.maybe true (U64.lte value) high)
-    |> ret
+val redeemRedemption: txSkeleton -> contractId -> sender -> redemption -> CR.t `cost` 2217 //(806 + 802 + 64 + 64 + 64 + 414 + 3)
+let redeemRedemption txSkel contractId sender redemption =
+    let! betToken = mkBetToken contractId redemption.bet in // 806
+    let! attestToken = mkAttestToken redemption.bet.event.oracleContractId redemption.attestation in // 802
+    let! m = TX.getAvailableTokens betToken txSkel in // 64
+    ret txSkel
+    >>= TX.destroy m betToken // 64
+    >>= TX.destroy 1UL attestToken // 64
+    >>= lockToSender Asset.zenAsset m sender // 414
+    >>= CR.ofTxSkel //3
 
-
-
+val redeem: txSkeleton -> contractId -> sender -> option data -> CR.t `cost` 111489 // (4 + 1700 + 107568 + 2217)
+let redeem txSkel contractId sender messageBody =
+    let open RT in
+    parseDict messageBody // 4
+    >>= parseRedemption // 1700
+    >>= validateRedemption // 107568
+    >>= redeemRedemption txSkel contractId sender // 2217
 
 (*
 -------------------------------------------------------------------------------
@@ -411,11 +517,14 @@ val main:
     -> messageBody : option data
     -> wallet      : wallet
     -> state       : option data
-    -> CR.t `cost` 2603
+    -> CR.t `cost` 111489
 let main txSkel context contractId command sender messageBody wallet state =
     match command with
     | "Buy" ->
         buy txSkel contractId sender messageBody
+        |> inc 108324
+    | "Redeem" ->
+        redeem txSkel contractId sender messageBody
     | _ ->
         RT.failw "Unsupported command"
-        |> inc 2603
+        |> inc 111489
